ulib/FStar.SizeT.fsti
@@ -57,6 +57,19 @@ val mul (x y: t) : Pure t
   (requires (fits (v x * v y)))
   (ensures (fun z -> v z == v x * v y))
 
+(** Modulo specification, similar to FStar.UInt.mod *)
+
+let mod_spec (a:nat{fits a}) (b:nat{fits b /\ b <> 0}) : GTot (n:nat{fits n}) =
+  let open FStar.Mul in
+  a - ((a/b) * b)
+
+(** Euclidean remainder
+
+    The result is the modulus of [a] with respect to a non-zero [b] *)
+val rem (a:t) (b:t{v b <> 0}) : Pure t
+  (requires True)
+  (ensures (fun c -> mod_spec (v a) (v b) = v c))
+
 (** Greater than *)
 val gt (x y:t) : Pure bool
   (requires True)
@@ -90,6 +103,7 @@ let one : (zero_size: t { v zero_size == 1 }) = mk 1us
 unfold let op_Plus_Hat = add
 unfold let op_Subtraction_Hat = sub
 unfold let op_Star_Hat = mul
+unfold let op_Percent_Hat = rem
 unfold let op_Greater_Hat = gt
 unfold let op_Greater_Equals_Hat = gte
 unfold let op_Less_Hat = lt
